Feat: Finalize function development

test/validate.py
@@ -1,5 +1,0 @@
-from eth2spec.capella import mainnet as spec
-from eth2spec.utils.ssz.ssz_typing import (uint64)
-
-x = uint64(16)
-assert spec.integer_squareroot(x) == 4
